@prefix : <https://w3id.org/olu/model#> .
@prefix qb: <http://purl.org/linked-data/cube#> .
@prefix dct: <http://purl.org/dc/terms/> .
@prefix owl: <http://www.w3.org/2002/07/owl#> .
@prefix rdf: <http://www.w3.org/1999/02/22-rdf-syntax-ns#> .
@prefix xml: <http://www.w3.org/XML/1998/namespace> .
@prefix xsd: <http://www.w3.org/2001/XMLSchema#> .
@prefix dcat: <http://www.w3.org/ns/dcat#> .
@prefix foaf: <http://xmlns.com/foaf/0.1/> .
@prefix prov: <http://www.w3.org/ns/prov#> .
@prefix rdfs: <http://www.w3.org/2000/01/rdf-schema#> .
@prefix skos: <http://www.w3.org/2004/02/skos/core#> .
@prefix stat: <http://data.europa.eu/m8g/> .
@prefix schema: <https://schema.org/> .
@prefix af-inspire:	<http://inspire.ec.europa.eu/schemas/af/3.0#> .
@prefix act-inspire:	<http://inspire.ec.europa.eu/schemas/act-core/3.0#> .
@prefix foodie: <http://foodie-cloud.com/model/foodie#> .
@prefix saref4agri: <https://w3id.org/def/saref4agri#> .
@prefix common: <http://portele.de/ont/inspire/baseInspire#> .
@prefix fiware: <https://uri.fiware.org/ns/data-models#> .
@prefix iso19109: <http://def.seegrid.csiro.au/isotc211/iso19109/2005/feature#> .
@prefix iso19150-2: <http://def.seegrid.csiro.au/isotc211/iso19150/-2/2012/basic#> .
@prefix iso19103: <http://def.seegrid.csiro.au/isotc211/iso19103/2005/basic#> .
@prefix geo:   <http://www.opengis.net/ont/geosparql#> .
@prefix ssn: <http://www.w3.org/ns/ssn/> .
@prefix sosa: <http://www.w3.org/ns/sosa/> .
@prefix saref: <https://w3id.org/saref#> .
@prefix gn: <https://www.geonames.org/ontology#> .
@prefix spatial: <http://geovocab.org/spatial#> .
@prefix lcc-country: <https://www.omg.org/spec/LCC/Countries/CountryRepresentation#> .
@prefix dcat: <http://www.w3.org/ns/dcat#> .
@prefix geo: <http://www.opengis.net/ont/geosparql#> .
@prefix ramon: <http://rdfdata.eionet.europa.eu/ramon/ontology/> .
@base <https://w3id.org/olu/model#> .

<https://w3id.org/olu/model> rdf:type owl:Ontology ;
                            owl:versionIRI <https://w3id.org/olu/model/1.0> ;
                            dct:creator [ schema:affiliation [ foaf:name "PSNC"
                                                             ] ;
                                          rdfs:seeAlso <http://orcid.org/0000-0003-4289-4922> ;
                                          foaf:name "Raul Palma"
                                        ] ;
                            dct:description "The Open Land Use (OLU) ontology has been derived from the SIEUSOIL OLU model version 2"@en ;
                            dct:rights "This vocabulary is distributed under Creative Commons Attribution 4.0 License - http://creativecommons.org/licenses/by/4.0"@en ;
                            dct:title "Open Land Use (OLU) ontology"@en ;
                            dct:source "OLU model version 2 - SIEUSOIL project" ;
                            rdfs:comment "The Open Land Use (OLU) ontology is the common vocabulary to represent land use data in SIEUSOIL project"@en ;
                            owl:versionInfo "1.0" ;
                            foaf:maker [ foaf:homepage <https://www.sieusoil.eu/> ;
                                         foaf:name "SIEUSOIL project"
                                       ] .

#################################################################
#    Annotation properties
#################################################################

dct:title rdf:type owl:AnnotationProperty ;
    rdfs:comment "A name given to the resource."@en ;
    rdfs:isDefinedBy <http://purl.org/dc/terms/> ;
    rdfs:label "Title"@en .
        
dct:description rdf:type owl:AnnotationProperty ;
    rdfs:comment "An account of the resource."@en ;
    rdfs:isDefinedBy <http://purl.org/dc/terms/> ;
    rdfs:label "Description"@en .   
    
#dct:source rdf:type rdf:Property ;
#    rdfs:comment "A related resource from which the described resource is derived."@en ;
#    rdfs:isDefinedBy <http://purl.org/dc/terms/> ;
#    rdfs:label "Source"@en .     

#################################################################
#    Datatypes
#################################################################


#################################################################
#    Object Properties
#################################################################

### http://purl.org/dc/terms/type
dct:type
    a owl:ObjectProperty ;
    rdfs:comment "The nature or genre of the resource."@en ;
    rdfs:isDefinedBy <http://purl.org/dc/terms/> ;
    rdfs:label "Type"@en . 

### http://www.opengis.net/ont/geosparql#hasGeometry
geo:hasGeometry
  a owl:ObjectProperty ;
  rdfs:range 	geo:Geometry ;
  rdfs:isDefinedBy geo: ;
  rdfs:comment " A spatial representation for a given feature. "@en ;  
  rdfs:label "hasGeometry"@en .  
  
### http://w3id.org/olu/model#attributeOrigin
:attributeOrigin
  a owl:ObjectProperty ;
  rdfs:isDefinedBy : ;
  rdfs:domain :AttributeSet ;
  rdfs:range 	:AttributeOriginCode ;
  rdfs:comment "Connects to the coded value representing the origin of the OLU attributes. It defines whether the set of attributes was imported together with OLUObject from the original dataset or related by model."@en ;  
  rdfs:label "attributeOrigin"@en .
  
### http://w3id.org/olu/model#originDataset
:originDataset
  a owl:ObjectProperty ;
  rdfs:domain [
  			owl:unionOf (
          :OLUObject
          :AttributeSet
        ) ] ;
  rdfs:isDefinedBy : ;
  rdfs:range 	:OriginDataset ;
  rdfs:comment "Connects to the dataset from which OLUObject, AttributeSet is originated when original dataset was imported in the model"@en ;  
  rdfs:label "originDataset"@en .  
  
### http://w3id.org/olu/model#oluTheme
:oluTheme
  a owl:ObjectProperty ;
  rdfs:isDefinedBy : ;
  rdfs:range 	:OLUTheme ;
  rdfs:domain :OriginDataset ;
  rdfs:comment "The related open land use theme"@en ;  
  rdfs:label "oluTheme"@en . 

### http://w3id.org/olu/model#hilucsValue
:hilucsValue
  a owl:ObjectProperty ;
  rdfs:isDefinedBy : ;
  rdfs:domain :AttributeSet ;
  rdfs:range 	skos:Concept ;
  rdfs:comment "The INSPIRE land use category"@en ;  
  rdfs:label "hilucsValue"@en . 

### http://w3id.org/olu/model#clcValue
:clcValue
  a owl:ObjectProperty ;
  rdfs:isDefinedBy : ;
  rdfs:domain :AttributeSet ;
  rdfs:range 	skos:Concept ;
  rdfs:comment "The Corine Land Cover category"@en ;  
  rdfs:label "clcValue"@en . 
  
### http://w3id.org/olu/model#administrativeUnit
:administrativeUnit
  a owl:ObjectProperty ;
  rdfs:subPropertyOf gn:parentFeature;
  rdfs:isDefinedBy : ;
#  rdfs:range 	:AdministrativeUnit ;
	rdfs:domain :OLUObject ;
	rdfs:range	ramon:NUTSRegion ;
  rdfs:comment "Connect to the NUTS region representing the related administrative unit"@en ;  
  rdfs:label "administrativeUnit"@en .    

### http://w3id.org/olu/model#relatedOLUObject
:relatedOLUObject
  a owl:ObjectProperty ;
  rdfs:isDefinedBy : ;
  rdfs:range 	:OLUObject ;
  rdfs:comment "The related OLUObject"@en ;  
  rdfs:label "relatedOLUObject"@en . 

### http://w3id.org/olu/model#relatedAttributeSet
:relatedAttributeSet
  a owl:ObjectProperty ;
  rdfs:isDefinedBy : ;
  rdfs:range 	:AttributeSet ;
  rdfs:comment "The related AttributeSet"@en ;  
  rdfs:label "relatedAttributeSet"@en . 



#################################################################
#    Data properties
#################################################################


### http://purl.org/dc/terms/identifier
dct:identifier
    a owl:DatatypeProperty ;
    skos:definition "An unambiguous reference to the resource within a given context."@en ;
		rdfs:comment "Recommended best practice is to identify the resource by means of a string conforming to a formal identification system."@en ;
    rdfs:isDefinedBy <http://purl.org/dc/terms/> ;
    rdfs:label "Identifier"@en .

# owl ontology defines it as objectproperty  
### https://schema.org/name
#schema:name
#  a owl:DatatypeProperty ;
#  rdfs:label "name"@en ;
#  rdfs:comment "The name of the item."@en ;
#  rdfs:isDefinedBy <https://schema.org/name> .

# owl ontology defines it as objectproperty
### https://schema.org/url
#schema:url
#  a owl:DatatypeProperty ;
#  rdfs:label "url"@en ;
#  rdfs:comment "The URL of the item."@en ;
#  rdfs:isDefinedBy <https://schema.org/url> .

###  https://schema.org/validFrom
schema:validFrom rdf:type owl:DatatypeProperty ;
								 rdfs:comment "The date when the item becomes valid."@en ;
								 rdfs:label "validFrom"@en ;
								 rdfs:isDefinedBy <https://schema.org/validFrom> .
  
###  https://schema.org/validThrough
schema:validThrough rdf:type owl:DatatypeProperty ;
								 rdfs:comment "The date after when the item is not valid. For example the end of an offer, salary period, or a period of opening hours."@en ;
								 rdfs:label "validThrough"@en ;
								 rdfs:isDefinedBy <https://schema.org/validThrough> .  
  
### http://w3id.org/olu/model#geometryType 
:geometryType 
  a owl:DatatypeProperty ;
  rdfs:isDefinedBy : ;
#  rdfs:range [
#  			a rdfs:Datatype ;
#  			owl:oneOf (
#          "vector"
#          "raster"
#        ) ] ;
  rdfs:comment "property defining origin dataset geometry format, e.g., vector or raster"@en ;  
  rdfs:label "geometryType"@en .

### http://w3id.org/olu/model#columnsNames
:columnsNames
  a owl:DatatypeProperty ;
  rdfs:isDefinedBy : ;
  rdfs:domain :OriginDataset ;
  rdfs:comment "The List of column names of the original dataset"@en ;  
  rdfs:label "columnsNames"@en . 

### http://w3id.org/olu/model#metadataAsXML
:metadataAsXML
  a owl:DatatypeProperty ;
  rdfs:isDefinedBy : ;
  rdfs:domain :OriginDataset ;
  rdfs:comment "The full XML representation of a dataset metadata in ISO 19115 format, e.g., metadata record from the metadata catalogue (produced by Micka dataset catalogue, in Micka-lite profile)"@en ;  
  rdfs:label "metadataAsXML"@en .    

### http://w3id.org/olu/model#attributes 
:attributes 
  a owl:DatatypeProperty ;
  rdfs:isDefinedBy : ;
  rdfs:domain :AttributeSet ;
  rdfs:comment "Set of other attributes of the OLUObject. It is a text containing additional attributes of an OLUObject as defined in an imported dataset, formatted in a set of key-value pairs"@en ;  
  rdfs:label "attributes "@en .  

### http://w3id.org/olu/model#zValue
:zValue
  a owl:DatatypeProperty ;
  rdfs:isDefinedBy : ;
  rdfs:comment "Number representing position of the feature in the stack of layers, small scale feature has lower value of z_value, large scale feature has larger value. The z-value defines the order of a particular object in the set of datasets."@en ;  
  rdfs:label "zValue"@en .

### http://w3id.org/olu/model#isReference
:isReference
  a owl:DatatypeProperty ;
  rdfs:isDefinedBy : ;
  rdfs:domain :OriginDataset ;
  rdfs:range xsd:boolean ;
  rdfs:comment "Defines whether the OriginDataset contains reference geometries or it contains thematic data imported to the model."@en ;  
  rdfs:label "isReference"@en .

### http://w3id.org/olu/model#originDescription
:originDescription
  a owl:DatatypeProperty ;
  rdfs:isDefinedBy : ;
  rdfs:range xsd:string ;
  rdfs:comment "Plain text description of origin of the Theme"@en ;  
  rdfs:label "originDescription"@en .  
  
                                                                        
#################################################################
#    Classes
#################################################################

### http://w3id.org/olu/model#OLUObject
:OLUObject	a owl:Class ;
			rdfs:subClassOf  gn:Feature, geo:Feature ;
      rdfs:subClassOf  [ a owl:Restriction ;
                           owl:cardinality  "1"^^xsd:int ;
                           owl:onProperty   		dct:identifier
                         ] ;
			rdfs:subClassOf  [ a owl:Restriction ;
                           owl:cardinality  "1"^^xsd:int ;
                           owl:onProperty   		geo:hasGeometry
                         ] ;
      rdfs:subClassOf  [ a owl:Restriction ;
                           owl:cardinality  "1"^^xsd:int ;
                           owl:onProperty   		:zValue
                         ] ;
      rdfs:subClassOf  [ a owl:Restriction ;
                           owl:maxCardinality  "1"^^xsd:int ;
                           owl:onProperty   		schema:validFrom
                         ] ;
			rdfs:subClassOf  [ a owl:Restriction ;
                           owl:maxCardinality  "1"^^xsd:int ;
                           owl:onProperty   		schema:validThrough
                         ] ;                             
      rdfs:subClassOf  [ a owl:Restriction ;
                           owl:cardinality  "1"^^xsd:int ;
                           owl:onProperty   		:originDataset
                         ] ;
      rdfs:subClassOf  [ a owl:Restriction ;
                           owl:minCardinality  "1"^^xsd:int ;
                           owl:onProperty   		:relatedAttributeSet
                         ] ;
      rdfs:subClassOf  [ a owl:Restriction ;
                           owl:minCardinality  "1"^^xsd:int ;
                           owl:onProperty   		:administrativeUnit
                         ] ;
			rdfs:label "OLUObject" ;   
			rdfs:comment "This class represents the main open land use (OLU) object, which has a geometry associated. It representats a real-world phenomenon in terms of land use theme with explicit localization" ;
			rdfs:isDefinedBy : . 
						
### http://w3id.org/olu/model#AttributeSet
:AttributeSet	a owl:Class ;
      rdfs:subClassOf  [ a owl:Restriction ;
                           owl:cardinality  "1"^^xsd:int ;
                           owl:onProperty   		dct:identifier
                         ] ;
      rdfs:subClassOf  [ a owl:Restriction ;
                           owl:cardinality  "1"^^xsd:int ;
                           owl:onProperty   		:attributes
                         ] ;                   
			rdfs:subClassOf  [ a owl:Restriction ;
                           owl:cardinality  "1"^^xsd:int ;
                           owl:onProperty   		:hilucsValue
                         ] ;
      rdfs:subClassOf  [ a owl:Restriction ;
                           owl:cardinality  "1"^^xsd:int ;
                           owl:onProperty   		:clcValue
                         ] ;
      rdfs:subClassOf  [ a owl:Restriction ;
                           owl:cardinality  "1"^^xsd:int ;
                           owl:onProperty   		:attributeOrigin
                         ] ;
      rdfs:subClassOf  [ a owl:Restriction ;
                           owl:allValuesFrom 	:AttributeOriginCode ;
                           owl:onProperty   	:attributeOrigin
                         ] ;                          
      rdfs:subClassOf  [ a owl:Restriction ;
                           owl:cardinality  "1"^^xsd:int ;
                           owl:onProperty   		:originDataset
                         ] ;
      rdfs:subClassOf  [ a owl:Restriction ;
                           owl:cardinality  "1"^^xsd:int ;
                           owl:onProperty   		:relatedOLUObject
                         ] ;                                                                      
			rdfs:label "AttributeSet" ;   
			rdfs:comment "This class represents the object for storing non-geometric attributes of OLUObjects" ;
			rdfs:isDefinedBy : .             
						
### http://w3id.org/olu/model#OriginDataset
:OriginDataset	a owl:Class ;
			rdfs:subClassOf  dcat:Dataset ;
      rdfs:subClassOf  [ a owl:Restriction ;
                           owl:cardinality  "1"^^xsd:int ;
                           owl:onProperty   		dct:identifier
                         ] ;
#      rdfs:subClassOf  [ a owl:Restriction ;
#                           owl:cardinality  "1"^^xsd:int ;
#                           owl:onProperty   		schema:url
#                         ] ;
      rdfs:subClassOf  [ a owl:Restriction ;
                           owl:allValuesFrom 	xsd:anyURI ;
                           owl:onProperty   		schema:url
                         ] ;                         
      rdfs:subClassOf  [ a owl:Restriction ;
                           owl:cardinality  "1"^^xsd:int ;
                           owl:onProperty   		dct:type
                         ] ;
      rdfs:subClassOf  [ a owl:Restriction ;
                           owl:allValuesFrom 	:DatasetTypeCode ;
                           owl:onProperty   		dct:type
                         ] ;                         
#      rdfs:subClassOf  [ a owl:Restriction ;
#                           owl:cardinality  "1"^^xsd:int ;
#                           owl:onProperty   		schema:name
#                         ] ;
      rdfs:subClassOf  [ a owl:Restriction ;
                           owl:allValuesFrom 	xsd:string ;
                           owl:onProperty   		schema:name
                         ] ;
			rdfs:subClassOf  [ a owl:Restriction ;
                           owl:maxCardinality  "1"^^xsd:int ;
                           owl:onProperty   		schema:validFrom
                         ] ;
			rdfs:subClassOf  [ a owl:Restriction ;
                           owl:maxCardinality  "1"^^xsd:int ;
                           owl:onProperty   		schema:validThrough
                         ] ; 
      rdfs:subClassOf  [ a owl:Restriction ;
                           owl:cardinality  "1"^^xsd:int ;
                           owl:onProperty   		:metadataAsXML
                         ] ;
      rdfs:subClassOf  [ a owl:Restriction ;
                           owl:cardinality  "1"^^xsd:int ;
                           owl:onProperty   		:geometryType 
                         ] ;   
			rdfs:subClassOf  [ a owl:Restriction ;
                           owl:allValuesFrom 	[ a rdfs:Datatype; owl:oneOf ("vector" "raster") ] ;
                           owl:onProperty   		:geometryType 
                         ] ;                                 
      rdfs:subClassOf  [ a owl:Restriction ;
                           owl:cardinality  "1"^^xsd:int ;
                           owl:onProperty   		:columnsNames
                         ] ; 
      rdfs:subClassOf  [ a owl:Restriction ;
                           owl:cardinality  "1"^^xsd:int ;
                           owl:onProperty   		:zValue
                         ] ;
      rdfs:subClassOf  [ a owl:Restriction ;
                           owl:cardinality  "1"^^xsd:int ;
                           owl:onProperty   		:isReference
                         ] ;
			rdfs:subClassOf  [ a owl:Restriction ;
                           owl:minCardinality  "1"^^xsd:int ;
                           owl:onProperty   		:oluTheme
                         ] ;
			                                                                                          
			rdfs:label "OriginDataset" ;   
			rdfs:comment "This class represents the dataset from where an OLU object was obtained and its metadata. This includes i) the original dataset imported to the data model containing representations of a real-world phenomena by geometric and non-geometric features; ii) the information describing spatial data sets and spatial data services, making it possible to discover, inventory and use them." ;
			rdfs:isDefinedBy : .			 			    

### http://w3id.org/olu/model#AdministrativeUnit
#:AdministrativeUnit	a owl:Class ;
#			rdfs:subClassOf  gn:Feature, geo:Feature, lcc-country:CountrySubdivision ;
#			rdfs:subClassOf  [ a owl:Restriction ;
#                           owl:minCardinality  "1"^^xsd:int ;
#                           owl:onProperty   		geo:hasGeometry
#                         ] ;
#      rdfs:subClassOf  [ a owl:Restriction ;
#                           owl:minCardinality  "1"^^xsd:int ;
#                           owl:onProperty   		ramon:name
#                         ] ;
#			rdfs:subClassOf  [ a owl:Restriction ;
#                           owl:minCardinality  "1"^^xsd:int ;
#                           owl:onProperty   		ramon:level
#                         ] ;
#      rdfs:subClassOf  [ a owl:Restriction ;
#                           owl:minCardinality  "1"^^xsd:int ;
#                           owl:onProperty   		ramon:code
#                         ] ;                         
#			rdfs:label "AdministrativeUnit" ;   
#			rdfs:comment "This class represents the administrative unit associated to the open land use object" ;
#			rdfs:isDefinedBy : .				
			
### http://w3id.org/olu/model#OLUTheme
:OLUTheme	a owl:Class ;
			rdfs:subClassOf  skos:Concept ;
			rdfs:subClassOf  [ a owl:Restriction ;
                           owl:cardinality  "1"^^xsd:int ;
                           owl:onProperty   		dct:identifier
                         ] ;
#      rdfs:subClassOf  [ a owl:Restriction ;
#                           owl:cardinality  "1"^^xsd:int ;
#                           owl:onProperty   		schema:name
#                         ] ;
      rdfs:subClassOf  [ a owl:Restriction ;
                           owl:allValuesFrom 	xsd:string ;
                           owl:onProperty   		schema:name
                         ] ;
      rdfs:subClassOf  [ a owl:Restriction ;
                           owl:cardinality  "1"^^xsd:int ;
                           owl:onProperty   		:originDescription
                         ] ;
#      rdfs:subClassOf  [ a owl:Restriction ;
#                           owl:cardinality  "1"^^xsd:int ;
#                           owl:onProperty   		schema:url
#                         ] ;
      rdfs:subClassOf  [ a owl:Restriction ;
                           owl:allValuesFrom 	xsd:anyURI ;
                           owl:onProperty   		schema:url
                         ] ;                         
			rdfs:label "OLUTheme" ;   
			rdfs:comment "This class represents the OLU object themes, typically connected to standard classifications, ontologies or well-known registries" ;
			rdfs:isDefinedBy : .	
			
### http://w3id.org/olu/model#AttributeOriginCode
:AttributeOriginCode	a owl:Class ;
			rdfs:subClassOf skos:Concept ;
			rdfs:label "Coded value list of sources for OLU attributes - codelist class"@en;
      rdfs:comment "This  code list provides the OLU attributes source."@en;
      rdfs:seeAlso :attributeOriginCode .			
			
			
### http://w3id.org/olu/model#attributeOriginCode
:attributeOriginCode	a skos:ConceptScheme;
			skos:prefLabel "Coded value list of sources for OLU attributes - codelist scheme"@en;
      rdfs:label "Code list for OLU attributes source - codelist scheme"@en;
      skos:note "This  code list provides the OLU attributes source."@en;
      rdfs:seeAlso :AttributeOriginCode .
      
### http://w3id.org/olu/model#DatasetTypeCode
:DatasetTypeCode	a owl:Class ;
			rdfs:subClassOf skos:Concept ;
			rdfs:label "Coded value list of types of Datasets - codelist class"@en;
      rdfs:comment "This  code list provides the Dataset types."@en;
      rdfs:seeAlso :datasetTypeCode .			
			
			
### http://w3id.org/olu/model#datasetTypeCode
:datasetTypeCode	a skos:ConceptScheme;
			skos:prefLabel "Coded value list of types of Datasets - codelist scheme"@en;
      rdfs:label "Code list for Dataseset types - codelist scheme"@en;
      skos:note "This  code list provides the Dataset types."@en;
      rdfs:seeAlso :DatasetTypeCode .      
			   
#################################################################
#    Alignments
#################################################################

#################################################################
#    Individuals
#################################################################

