@prefix : <https://w3id.org/olu/model#> .
@prefix qb: <http://purl.org/linked-data/cube#> .
@prefix dct: <http://purl.org/dc/terms/> .
@prefix owl: <http://www.w3.org/2002/07/owl#> .
@prefix rdf: <http://www.w3.org/1999/02/22-rdf-syntax-ns#> .
@prefix xml: <http://www.w3.org/XML/1998/namespace> .
@prefix xsd: <http://www.w3.org/2001/XMLSchema#> .
@prefix dcat: <http://www.w3.org/ns/dcat#> .
@prefix foaf: <http://xmlns.com/foaf/0.1/> .
@prefix prov: <http://www.w3.org/ns/prov#> .
@prefix rdfs: <http://www.w3.org/2000/01/rdf-schema#> .
@prefix skos: <http://www.w3.org/2004/02/skos/core#> .
@prefix stat: <http://data.europa.eu/m8g/> .
@prefix schema: <https://schema.org/> .
@prefix af-inspire:	<http://inspire.ec.europa.eu/schemas/af/3.0#> .
@prefix act-inspire:	<http://inspire.ec.europa.eu/schemas/act-core/3.0#> .
@prefix foodie: <http://foodie-cloud.com/model/foodie#> .
@prefix saref4agri: <https://w3id.org/def/saref4agri#> .
@prefix common: <http://portele.de/ont/inspire/baseInspire#> .
@prefix fiware: <https://uri.fiware.org/ns/data-models#> .
@prefix iso19109: <http://def.seegrid.csiro.au/isotc211/iso19109/2005/feature#> .
@prefix iso19150-2: <http://def.seegrid.csiro.au/isotc211/iso19150/-2/2012/basic#> .
@prefix iso19103: <http://def.seegrid.csiro.au/isotc211/iso19103/2005/basic#> .
@prefix geo:   <http://www.opengis.net/ont/geosparql#> .
@prefix ssn: <http://www.w3.org/ns/ssn/> .
@prefix sosa: <http://www.w3.org/ns/sosa/> .
@prefix saref: <https://w3id.org/saref#> .
@prefix gn: <https://www.geonames.org/ontology#> .
@prefix spatial: <http://geovocab.org/spatial#> .
@prefix lcc-country: <https://www.omg.org/spec/LCC/Countries/CountryRepresentation#> .
@prefix dcat: <http://www.w3.org/ns/dcat#> .
@prefix geo: <http://www.opengis.net/ont/geosparql#> .
@prefix ramon: <http://rdfdata.eionet.europa.eu/ramon/ontology/> .
@base <https://w3id.org/olu/model#> .

<https://w3id.org/olu/model> rdf:type owl:Ontology ;
                            owl:versionIRI <https://w3id.org/olu/model/1.0> ;
                            dct:creator [ schema:affiliation [ foaf:name "PSNC"
                                                             ] ;
                                          rdfs:seeAlso <http://orcid.org/0000-0003-4289-4922> ;
                                          foaf:name "Raul Palma"
                                        ] ;
                            dct:description "The Open Land Use (OLU) ontology has been derived from the SIEUSOIL OLU model version 2"@en ;
                            dct:rights "This vocabulary is distributed under Creative Commons Attribution 4.0 License - http://creativecommons.org/licenses/by/4.0"@en ;
                            dct:title "Open Land Use (OLU) ontology"@en ;
                            dct:source "OLU model version 2 - SIEUSOIL project" ;
                            rdfs:comment "The Open Land Use (OLU) ontology is the common vocabulary to represent land use data in SIEUSOIL project"@en ;
                            owl:versionInfo "1.0" ;
                            foaf:maker [ foaf:homepage <https://www.sieusoil.eu/> ;
                                         foaf:name "SIEUSOIL project"
                                       ] .

#################################################################
#    Annotation properties
#################################################################

dct:title rdf:type owl:AnnotationProperty ;
    rdfs:comment "A name given to the resource."@en ;
    rdfs:isDefinedBy <http://purl.org/dc/terms/> ;
    rdfs:label "Title"@en .
        
dct:description rdf:type owl:AnnotationProperty ;
    rdfs:comment "An account of the resource."@en ;
    rdfs:isDefinedBy <http://purl.org/dc/terms/> ;
    rdfs:label "Description"@en .   
    
dct:source rdf:type owl:AnnotationProperty ;
    rdfs:comment "A related resource from which the described resource is derived."@en ;
    rdfs:isDefinedBy <http://purl.org/dc/terms/> ;
    rdfs:label "Source"@en .     

#################################################################
#    Datatypes
#################################################################


#################################################################
#    Object Properties
#################################################################

### http://purl.org/dc/terms/type
dct:type
    a owl:ObjectProperty ;
    rdfs:comment "The nature or genre of the resource."@en ;
    rdfs:isDefinedBy <http://purl.org/dc/terms/> ;
    rdfs:label "Type"@en . 

### https://schema.org/name
schema:name
  a owl:ObjectProperty ;
  rdfs:label "name"@en ;
  rdfs:comment "The name of the item."@en ;
  rdfs:isDefinedBy <https://schema.org/name> .

### http://www.opengis.net/ont/geosparql#hasGeometry
geo:hasGeometry
  a owl:ObjectProperty ;
  rdfs:isDefinedBy geo: ;
  rdfs:comment " A spatial representation for a given feature. "@en ;  
  rdfs:label "hasGeometry"@en .  
  
### http://w3id.org/olu/model#attributeOrigin
:attributeOrigin
  a owl:ObjectProperty ;
  rdfs:isDefinedBy : ;
  rdfs:domain :OLUObject ;
  rdfs:range 	:AttributeOriginCode ;
  rdfs:comment "Connects to the coded value representing the origin of the OLU attributes"@en ;  
  rdfs:label "attributeOrigin"@en .
  
### http://w3id.org/olu/model#originDataset
:originDataset
  a owl:ObjectProperty ;
  rdfs:domain :OLUObject ; 
  rdfs:isDefinedBy : ;
  rdfs:range 	:OriginDataset ;
  rdfs:comment "Connects to the dataset from which the object was obtained"@en ;  
  rdfs:label "originDataset"@en .  
  
### http://w3id.org/olu/model#hilucsValue
:hilucsValue
  a owl:ObjectProperty ;
  rdfs:isDefinedBy : ;
  rdfs:domain :OLUObject ;
  rdfs:range 	skos:Concept ;
  rdfs:comment "The INSPIRE land use category"@en ;  
  rdfs:label "hilucsValue"@en . 
  
### http://w3id.org/olu/model#oluTheme
:oluTheme
  a owl:ObjectProperty ;
  rdfs:isDefinedBy : ;
  rdfs:range 	:OLUTheme ;
  rdfs:domain [
  			owl:unionOf (
          :OriginDataset
          :OLUObject
        ) ] ;
  rdfs:comment "The related open land use theme"@en ;  
  rdfs:label "oluTheme"@en . 
  
### http://w3id.org/olu/model#administrativeUnit
:administrativeUnit
  a owl:ObjectProperty ;
  rdfs:subPropertyOf gn:parentFeature;
  rdfs:isDefinedBy : ;
#  rdfs:range 	:AdministrativeUnit ;
	rdfs:domain :OLUObject ;
	rdfs:range	ramon:NUTSRegion ;
  rdfs:comment "Connect to the NUTS region representing the related administrative unit"@en ;  
  rdfs:label "administrativeUnit"@en .    

#################################################################
#    Data properties
#################################################################

### http://purl.org/dc/terms/identifier
dct:identifier
    a owl:DatatypeProperty ;
    skos:definition "An unambiguous reference to the resource within a given context."@en ;
		rdfs:comment "Recommended best practice is to identify the resource by means of a string conforming to a formal identification system."@en ;
    rdfs:isDefinedBy <http://purl.org/dc/terms/> ;
    rdfs:label "Identifier"@en .
  
###  https://schema.org/validFrom
schema:validFrom rdf:type owl:DatatypeProperty ;
								 rdfs:comment "The date when the item becomes valid."@en ;
								 rdfs:label "validFrom"@en ;
								 rdfs:isDefinedBy <https://schema.org/validFrom> .
  
###  https://schema.org/validThrough
schema:validThrough rdf:type owl:DatatypeProperty ;
								 rdfs:comment "The date after when the item is not valid. For example the end of an offer, salary period, or a period of opening hours."@en ;
								 rdfs:label "validThrough"@en ;
								 rdfs:isDefinedBy <https://schema.org/validThrough> .  
  
### http://w3id.org/olu/model#originGeoFormat
:originGeoFormat
  a owl:DatatypeProperty ;
  rdfs:isDefinedBy : ;
#  rdfs:range [
#  			a rdfs:Datatype ;
#  			owl:oneOf (
#          "vector"
#          "raster"
#        ) ] ;
  rdfs:comment "property defining origin dataset geometry format, e.g., vector or raster"@en ;  
  rdfs:label "originGeoFormat"@en .

### http://w3id.org/olu/model#zValue
:zValue
  a owl:DatatypeProperty ;
  rdfs:isDefinedBy : ;
  rdfs:comment "Number representing position of the feature in the stack of layers, small scale feature has lower value of z_value, large scale feature has larger value"@en ;  
  rdfs:label "zValue"@en .
  
### http://w3id.org/olu/model#nonGeoAttributesAsJson
:nonGeoAttributesAsJson
  a owl:DatatypeProperty ;
  rdfs:isDefinedBy : ;
  rdfs:domain :OLUObject ;
  rdfs:comment "The JSON representation of OLU non-geometric attributes, which came from one original dataset or were generated by one algorithm/function"@en ;  
  rdfs:label "attributeAsJson"@en .  

### http://w3id.org/olu/model#columnsAsJson
:columnsAsJson
  a owl:DatatypeProperty ;
  rdfs:isDefinedBy : ;
  rdfs:domain :OriginDataset ;
  rdfs:comment "The JSON representation of column names of the origin dataset"@en ;  
  rdfs:label "columnsAsJson"@en . 
  
### http://w3id.org/olu/model#metadataAsXML
:metadataAsXML
  a owl:DatatypeProperty ;
  rdfs:isDefinedBy : ;
  rdfs:domain :OriginDataset ;
  rdfs:comment "The full XML representation of a dataset metadata in ISO 19115 format"@en ;  
  rdfs:label "metadataAsXML"@en .    
                 
                                                                        
#################################################################
#    Classes
#################################################################

### http://w3id.org/olu/model#OLUObject
:OLUObject	a owl:Class ;
			rdfs:subClassOf  gn:Feature, geo:Feature ;
			rdfs:subClassOf  [ a owl:Restriction ;
                           owl:minCardinality  "1"^^xsd:int ;
                           owl:onProperty   		geo:hasGeometry
                         ] ;
      rdfs:subClassOf  [ a owl:Restriction ;
                           owl:minCardinality  "1"^^xsd:int ;
                           owl:onProperty   		:zValue
                         ] ;
      rdfs:subClassOf  [ a owl:Restriction ;
                           owl:minCardinality  "1"^^xsd:int ;
                           owl:onProperty   		:originDataset
                         ] ;
      rdfs:subClassOf  [ a owl:Restriction ;
                           owl:minCardinality  "1"^^xsd:int ;
                           owl:onProperty   		:administrativeUnit
                         ] ;
      rdfs:subClassOf  [ a owl:Restriction ;
                           owl:minCardinality  "1"^^xsd:int ;
                           owl:onProperty   		:oluTheme
                         ] ;
      rdfs:subClassOf  [ a owl:Restriction ;
                           owl:minCardinality  "1"^^xsd:int ;
                           owl:onProperty   		:nonGeoAttributesAsJson
                         ] ;                   
			rdfs:subClassOf  [ a owl:Restriction ;
                           owl:minCardinality  "1"^^xsd:int ;
                           owl:onProperty   		:hilucsValue
                         ] ;
      rdfs:subClassOf  [ a owl:Restriction ;
                           owl:minCardinality  "1"^^xsd:int ;
                           owl:onProperty   		:attributeOrigin
                         ] ;                                                                     
			rdfs:label "OLUObject" ;   
			rdfs:comment "This class represents the main open land use (OLU) object, which has associated both geometric and non-geometric properties" ;
			rdfs:isDefinedBy : . 
						
						
### http://w3id.org/olu/model#OriginDataset
:OriginDataset	a owl:Class ;
			rdfs:subClassOf  dcat:Dataset ;
			rdfs:subClassOf  [ a owl:Restriction ;
                           owl:minCardinality  "1"^^xsd:int ;
                           owl:onProperty   		schema:name
                         ] ;
			rdfs:subClassOf  [ a owl:Restriction ;
                           owl:minCardinality  "1"^^xsd:int ;
                           owl:onProperty   		dct:identifier
                         ] ;
			rdfs:subClassOf  [ a owl:Restriction ;
                           owl:minCardinality  "1"^^xsd:int ;
                           owl:onProperty   		dct:type
                         ] ;
			rdfs:subClassOf  [ a owl:Restriction ;
                           owl:allValuesFrom 	:DatasetTypeCode ;
                           owl:onProperty   		dct:type
                         ] ;                         
			rdfs:subClassOf  [ a owl:Restriction ;
                           owl:minCardinality  "1"^^xsd:int ;
                           owl:onProperty   		schema:validFrom
                         ] ;
			rdfs:subClassOf  [ a owl:Restriction ;
                           owl:minCardinality  "1"^^xsd:int ;
                           owl:onProperty   		schema:validThrough
                         ] ;    
      rdfs:subClassOf  [ a owl:Restriction ;
                           owl:minCardinality  "1"^^xsd:int ;
                           owl:onProperty   		:columnsAsJson
                         ] ; 
      rdfs:subClassOf  [ a owl:Restriction ;
                           owl:minCardinality  "1"^^xsd:int ;
                           owl:onProperty   		:metadataAsXML
                         ] ;
      rdfs:subClassOf  [ a owl:Restriction ;
                           owl:minCardinality  "1"^^xsd:int ;
                           owl:onProperty   		:zValue
                         ] ;
			rdfs:subClassOf  [ a owl:Restriction ;
                           owl:minCardinality  "1"^^xsd:int ;
                           owl:onProperty   		:oluTheme
                         ] ;
			rdfs:subClassOf  [ a owl:Restriction ;
                           owl:minCardinality  "1"^^xsd:int ;
                           owl:onProperty   		:originGeoFormat
                         ] ;   
			rdfs:subClassOf  [ a owl:Restriction ;
                           owl:allValuesFrom 	[ a rdfs:Datatype; owl:oneOf ("vector" "raster") ] ;
                           owl:onProperty   		:originGeoFormat
                         ] ;                                                                                          
			rdfs:label "OriginDataset" ;   
			rdfs:comment "This class represents the dataset from where an OLU object was obtained" ;
			rdfs:isDefinedBy : .			 			    

### http://w3id.org/olu/model#AdministrativeUnit
#:AdministrativeUnit	a owl:Class ;
#			rdfs:subClassOf  gn:Feature, geo:Feature, lcc-country:CountrySubdivision ;
#			rdfs:subClassOf  [ a owl:Restriction ;
#                           owl:minCardinality  "1"^^xsd:int ;
#                           owl:onProperty   		geo:hasGeometry
#                         ] ;
#      rdfs:subClassOf  [ a owl:Restriction ;
#                           owl:minCardinality  "1"^^xsd:int ;
#                           owl:onProperty   		ramon:name
#                         ] ;
#			rdfs:subClassOf  [ a owl:Restriction ;
#                           owl:minCardinality  "1"^^xsd:int ;
#                           owl:onProperty   		ramon:level
#                         ] ;
#      rdfs:subClassOf  [ a owl:Restriction ;
#                           owl:minCardinality  "1"^^xsd:int ;
#                           owl:onProperty   		ramon:code
#                         ] ;                         
#			rdfs:label "AdministrativeUnit" ;   
#			rdfs:comment "This class represents the administrative unit associated to the open land use object" ;
#			rdfs:isDefinedBy : .				
			
### http://w3id.org/olu/model#OLUTheme
:OLUTheme	a owl:Class ;
			rdfs:subClassOf  skos:Concept ;
			rdfs:subClassOf  [ a owl:Restriction ;
                           owl:minCardinality  "1"^^xsd:int ;
                           owl:onProperty   		dct:identifier
                         ] ;
      rdfs:subClassOf  [ a owl:Restriction ;
                           owl:minCardinality  "1"^^xsd:int ;
                           owl:onProperty   		schema:name
                         ] ;
			rdfs:label "OLUTheme" ;   
			rdfs:comment "This class represents the OLU object themes, typically connected to standard classifications, ontologies or well-known registries" ;
			rdfs:isDefinedBy : .	
			
### http://w3id.org/olu/model#AttributeOriginCode
:AttributeOriginCode	a owl:Class ;
			rdfs:subClassOf skos:Concept ;
			rdfs:label "Coded value list of sources for OLU attributes - codelist class"@en;
      rdfs:comment "This  code list provides the OLU attributes source."@en;
      rdfs:seeAlso :attributeOriginCode .			
			
			
### http://w3id.org/olu/model#attributeOriginCode
:attributeOriginCode	a skos:ConceptScheme;
			skos:prefLabel "Coded value list of sources for OLU attributes - codelist scheme"@en;
      rdfs:label "Code list for OLU attributes source - codelist scheme"@en;
      skos:note "This  code list provides the OLU attributes source."@en;
      rdfs:seeAlso :AttributeOriginCode .
      
### http://w3id.org/olu/model#DatasetTypeCode
:DatasetTypeCode	a owl:Class ;
			rdfs:subClassOf skos:Concept ;
			rdfs:label "Coded value list of types of Datasets - codelist class"@en;
      rdfs:comment "This  code list provides the Dataset types."@en;
      rdfs:seeAlso :datasetTypeCode .			
			
			
### http://w3id.org/olu/model#datasetTypeCode
:datasetTypeCode	a skos:ConceptScheme;
			skos:prefLabel "Coded value list of types of Datasets - codelist scheme"@en;
      rdfs:label "Code list for Dataseset types - codelist scheme"@en;
      skos:note "This  code list provides the Dataset types."@en;
      rdfs:seeAlso :DatasetTypeCode .      
			   
#################################################################
#    Alignments
#################################################################

#################################################################
#    Individuals
#################################################################

